src/coq/Syntax/Scope.v
@@ -1,0 +1,144 @@
+(* begin hide *)
+From Coq Require Import
+     List.
+Import ListNotations.
+
+From Vellvm Require Import
+     Numeric.Coqlib
+     Syntax.LLVMAst
+     Syntax.CFG
+     Syntax.TypToDtyp.
+(* end hide *)
+
+(** * Scoping
+    We define through this file several functions and predicates having to do with the scope
+    of VIR programs, w.r.t. both block identifiers and local variables.
+    We unfortunately inherit from LLVM IR a fully named representation of variables, forcing
+    on us fairly heavy sanity checks.
+    - [inputs]: input labels of an [ocfg]
+    - [outputs]: output labels of an [ocfg]
+    - [wf_ocfg_bid]: no duplicate block identifiers
+
+
+ *)
+
+(** * Well-formedness w.r.t. block identifiers
+    An [ocfg] should not admit any collisions w.r.t. to its labels.
+ *)
+Section OCFG_BID_OPERATIONS.
+
+  Context {T : Type}.
+
+  (** * inputs
+     Collect the list of input labels in an open control flow graph.
+     Denoting an [ocfg] starting from a label out of this static list
+     always results in the identity.
+   *)
+  Definition inputs {t} (ocfg : @ocfg t) :=
+    map blk_id ocfg.
+
+  (** * outputs
+     Collect the list of output labels in an open control flow graph.
+     Denoting an [ocfg] starting from a label that belongs to its [inputs]
+     will always result in a label in the static [output] list, or in a value.
+   *)
+  Definition terminator_outputs {t} (term : LLVMAst.terminator t) : list block_id
+    := match term with
+       | TERM_Ret v => []
+       | TERM_Ret_void => []
+       | TERM_Br v br1 br2 => [br1; br2]
+       | TERM_Br_1 br => [br]
+       | TERM_Switch v default_dest brs => default_dest :: map snd brs
+       | TERM_IndirectBr v brs => brs
+       | TERM_Resume v => []
+       | TERM_Invoke fnptrval args to_label unwind_label => [to_label; unwind_label]
+       end.
+
+  Definition bk_outputs {t} (bk : block t) : list block_id :=
+    terminator_outputs (snd (blk_term bk)).
+
+  Definition outputs {t} (bks : @ocfg t) : List.list block_id
+    := fold_left (fun acc bk => acc ++ bk_outputs bk) bks [].
+
+  (* All labels in a list of blocks are distinct *)
+  Definition wf_ocfg_bid {T} (bks : list (LLVMAst.block T)) :=
+    list_norepet (map blk_id bks).
+
+  (* The  *)
+  Lemma wf_ocfg_bid_nil:
+    forall T, wf_ocfg_bid (T := T) []. 
+  Proof.
+    intros; apply list_norepet_nil.
+  Qed.
+
+  Lemma wf_ocfg_bid_cons :
+    forall T (b : LLVMAst.block T) bs,
+      wf_ocfg_bid (b :: bs) ->
+      wf_ocfg_bid bs.
+  Proof.
+    intros * NOREP; inv NOREP; eauto.
+  Qed.
+
+  Lemma wf_ocfg_bid_cons_not_in :
+    forall T (b : LLVMAst.block T) bs,
+      wf_ocfg_bid (b :: bs) ->
+      not (In (blk_id b) (map blk_id bs)).
+  Proof.
+    intros * NOREP; inv NOREP; eauto.
+  Qed.
+
+  Lemma wf_ocfg_bid_app_r :
+    forall T (bs1 bs2 : list (LLVMAst.block T)), 
+      wf_ocfg_bid (bs1 ++ bs2) ->
+      wf_ocfg_bid bs2.
+  Proof.
+    intros * NR.
+    eapply list_norepet_append_right.
+    unfold wf_ocfg_bid in NR.
+    rewrite map_app in NR.
+    eauto.
+  Qed.
+
+  Lemma wf_ocfg_bid_app_l :
+    forall T (bs1 bs2 : list (LLVMAst.block T)), 
+      wf_ocfg_bid (bs1 ++ bs2) ->
+      wf_ocfg_bid bs1.
+  Proof.
+    intros * NR.
+    eapply list_norepet_append_left.
+    unfold wf_ocfg_bid in NR.
+    rewrite map_app in NR.
+    eauto.
+  Qed.
+
+  Lemma blk_id_convert_typ : forall env b,
+      blk_id (convert_typ env b) = blk_id b.
+  Proof.
+    intros ? []; reflexivity.
+  Qed.
+
+  (* Lemma blk_id_map_convert_typ : forall env bs, *)
+  (*     map blk_id (convert_typ env bs) = map blk_id bs. *)
+  (* Proof. *)
+  (*   induction bs as [| b bs IH]; cbn; auto. *)
+  (*   f_equal; auto. *)
+  (* Qed. *)
+
+  (* Lemma wf_ocfg_bid_convert_typ : *)
+  (*   forall env (bs : list (LLVMAst.block typ)), *)
+  (*     wf_ocfg_bid bs -> *)
+  (*     wf_ocfg_bid (convert_typ env bs). *)
+  (* Proof. *)
+  (*   induction bs as [| b bs IH]; intros NOREP. *)
+  (*   - cbn; auto. *)
+  (*   - cbn. *)
+  (*     apply list_norepet_cons.  *)
+  (*     + cbn. *)
+  (*       apply wf_ocfg_bid_cons_not_in in NOREP. *)
+  (*       rewrite blk_id_map_convert_typ; auto. *)
+  (*     + eapply IH, wf_ocfg_bid_cons; eauto.  *)
+  (* Qed. *)
+
+End OCFG_BID_OPERATIONS.
+
+
